theories/Subst.v
@@ -2,9 +2,9 @@ From Coq Require Import
   Lists.List.
 Import ListNotations.
 From Lang Require Import
+  DupFrom
   FreeVariables
   Invert
-  Mint
   Terms.
 
 Fixpoint smap
@@ -62,9 +62,20 @@ Proof.
   destruct a. simpl. destruct (eqb x s) eqn:E. { reflexivity. } simpl. reflexivity.
 Qed.
 
+Lemma remove_key_all_eq : forall {T} x li,
+  ~In x (map fst li) ->
+  @remove_key_all T x li = li.
+Proof.
+  intros. generalize dependent x. induction li; intros; simpl in *. { reflexivity. }
+  destruct a. simpl in *. apply Decidable.not_or in H as [H1 H2]. apply eqb_neq in H1.
+  rewrite eqb_sym in H1. rewrite H1. f_equal. apply IHli. assumption.
+Qed.
+
+Definition fst_cmp {A B} := fun (a : string * A) (b : string * B) => eqb (fst a) (fst b).
+
 (* Ludicrous that this is the easiest correct definition to write.
  * Generates substitution functions for every free variable at once. *)
-Fixpoint grand_unified_subst t : list (string * (term -> term)) :=
+Fixpoint grand_unified_subst_with rm t : list (string * (term -> term)) :=
   match t with
   | TmVoid
   | TmStar _
@@ -73,27 +84,29 @@ Fixpoint grand_unified_subst t : list (string * (term -> term)) :=
   | TmVarS s =>
       [(s, fun x => x)]
   | TmPack id arg ty curry =>
-      smap (fun f x => TmPack id arg (f x) curry) (grand_unified_subst ty) ++
-      smap (fun f x => TmPack id arg ty (f x)) (
-        let recursed := grand_unified_subst curry in
+      dup_from_src_with fst_cmp
+      (smap (fun f x => TmPack id arg (f x) curry) (grand_unified_subst_with remove_key_all ty))
+      (smap (fun f x => TmPack id arg ty (f x)) (
+        let recursed := grand_unified_subst_with rm curry in
         match arg with
         | None => recursed
-        | Some a =>
-            (if mint ty then remove_key_all else remove_key_if_head) a recursed
-        end)
+        | Some a => rm a recursed
+        end))
   | TmForA arg ty body =>
-      smap (fun f x => TmForA arg (f x) body) (grand_unified_subst ty) ++
-      smap (fun f x => TmForA arg ty (f x)) (
-        let recursed := grand_unified_subst body in
+      dup_from_src_with fst_cmp
+      (smap (fun f x => TmForA arg (f x) body) (grand_unified_subst_with remove_key_all ty))
+      (smap (fun f x => TmForA arg ty (f x)) (
+        let recursed := grand_unified_subst_with rm body in
         match arg with
         | None => recursed
-        | Some a =>
-            (if mint ty then remove_key_all else remove_key_if_head) a recursed
-        end)
+        | Some a => rm a recursed
+        end))
   | TmAppl a b =>
-      smap (fun f x => TmAppl (f x) b) (grand_unified_subst a) ++
-      smap (fun f x => TmAppl a (f x)) (grand_unified_subst b)
+      smap (fun f x => TmAppl (f x) b) (grand_unified_subst_with rm a) ++
+      smap (fun f x => TmAppl a (f x)) (grand_unified_subst_with rm b)
   end.
+Definition grand_unified_subst := grand_unified_subst_with remove_key_if_head.
+Arguments grand_unified_subst/ t.
 
 Fixpoint pair_lookup {V} key (pairs : list (string * V)) :=
   match pairs with
@@ -121,14 +134,80 @@ Example grand_unified_subst_lambda :
     ("x", fun x => TmForA (Some "x") (TmVarS "T") (TmAppl (TmVarS "x") x))]%string.
 Proof. reflexivity. Qed.
 
-Theorem grand_unified_subst_exactly_fv : forall t,
+Lemma has_cmp_fst : forall {T} li s t,
+  has_with (@fst_cmp T T) (s, t) li = has_with eqb s (map fst li).
+Proof.
+  intros T li. induction li; intros; simpl in *. { reflexivity. }
+  destruct a. unfold fst_cmp. simpl in *. destruct (eqb s s0). { reflexivity. }
+  apply IHli.
+Qed.
+
+Lemma has_fst_or : forall {T} x a b,
+  @has_with (string * T) (string * T) fst_cmp x (dup_from_src_with fst_cmp a b) =
+  orb (has_with fst_cmp x a) (has_with fst_cmp x b).
+Proof.
+  intros T x a. generalize dependent x. induction a; intros; simpl in *. { reflexivity. }
+  destruct (has_with fst_cmp a (dup_from_src_with fst_cmp a0 b)) eqn:Eh; simpl in *;
+  (destruct (fst_cmp x a) eqn:Ef; simpl in *; [| apply IHa]). 2: reflexivity.
+  destruct a. destruct x. rewrite has_cmp_fst in *.
+  unfold fst_cmp in Ef. simpl in *. apply eqb_eq in Ef. subst. assumption.
+Qed.
+
+Lemma dup_from_src_fst : forall {T} a b,
+  map fst (dup_from_src_with fst_cmp a b) = dup_from_src_with eqb (map (@fst _ T) a) (map fst b).
+Proof.
+  intros T a. induction a; intros; simpl in *. { reflexivity. }
+  destruct a. simpl in *. rewrite has_cmp_fst. rewrite IHa.
+  destruct (has_with eqb s (dup_from_src_with eqb (map fst a0) (map fst b)));
+  [| simpl in *; f_equal]; apply IHa.
+Qed.
+
+Lemma dup_from_src_nil_exists : forall {T} a b, exists pre,
+  dup_from_src_with (@fst_cmp _ T) a b = pre ++ b.
+Proof.
+  induction a; intros; simpl in *. { exists []. reflexivity. }
+  destruct (has_with fst_cmp a (dup_from_src_with fst_cmp a0 b)). { apply IHa. }
+  destruct (IHa b) as [x H]. exists (a :: x). simpl. f_equal. assumption.
+Qed.
+
+Fixpoint set_diff {T} (a b : list (string * T)) :=
+  match a with
+  | [] => []
+  | hd :: tl =>
+      let recursed := set_diff tl b in
+      if has_with fst_cmp hd b then recursed else hd :: recursed
+  end.
+
+Lemma dup_from_src_nil : forall {T} a b,
+  dup_from_src_with (@fst_cmp _ T) a b = set_diff a b ++ b.
+Proof.
+  induction a; intros; simpl in *. { reflexivity. }
+  destruct (has_with fst_cmp a (dup_from_src_with fst_cmp a0 b)) eqn:Eh;
+  rewrite has_fst_or in Eh; rewrite IHa; [| rewrite app_comm_cons]; f_equal.
+  - apply Bool.orb_prop in Eh. destruct Eh; [| rewrite H; reflexivity].
+    + admit.
+    + rewrite H.
+
+  destruct (has_with fst_cmp a b) eqn:Eh; rewrite has_fst_or; rewrite Eh. { rewrite Bool.orb_true_r. apply IHa. }
+  destruct (has_with fst_cmp a a0) eqn:E0; simpl in *; rewrite IHa; rewrite app_comm_cons; f_equal.
+Qed.
+
+Theorem grand_unified_subst_structural_fv : forall t,
+  fv_with remove_all t = map fst (grand_unified_subst_with remove_key_all t).
+Proof.
+  induction t; intros; subst; simpl in *; try reflexivity;
+  repeat rewrite IHt1; repeat rewrite IHt2; [| | repeat rewrite map_distr; repeat rewrite map_fst_smap; reflexivity];
+  destruct arg; repeat rewrite <- remove_all_key_eq; rewrite dup_from_src_fst; repeat rewrite map_fst_smap; reflexivity.
+Qed.
+
+Theorem grand_unified_subst_fv : forall t,
   fv t = map fst (grand_unified_subst t).
 Proof.
-  intros t. induction t; intros; subst; simpl in *; try reflexivity;
-  repeat rewrite IHt1; repeat rewrite IHt2; try destruct arg; destruct (reflect_mint t1);
-  repeat rewrite map_distr; repeat rewrite map_fst_smap; f_equal;
-  try (symmetry; apply remove_all_key_eq); destruct (grand_unified_subst t2); try reflexivity;
-  destruct p; simpl; destruct (eqb s s0); reflexivity.
+  induction t; intros; subst; simpl in *; try reflexivity;
+  repeat rewrite IHt1; repeat rewrite IHt2; [| | rewrite map_distr; repeat rewrite map_fst_smap; reflexivity];
+  rewrite dup_from_src_fst; repeat rewrite map_fst_smap; rewrite grand_unified_subst_structural_fv;
+  (destruct arg; [| reflexivity]); (destruct (grand_unified_subst_with remove_key_if_head t2) eqn:Eg; [reflexivity |]);
+  destruct p; simpl in *; (destruct (eqb s s0); reflexivity).
 Qed.
 (* WOOHOOOOOOOOOOOOOOO *)
 
@@ -196,10 +275,113 @@ Proof.
   unfold incl. intros T x [] [a1 a2] H. { inversion H. } destruct p. simpl in H. destruct (eqb x s); [right |]; assumption.
 Qed.
 
+(* God this is the dumbest function of all time but it's only ever used in proofs *)
+Fixpoint slow_unique_key {T} (li : list (string * T)) :=
+  match li with
+  | [] => []
+  | (s, t) :: tl => (s, t) :: remove_key_all s (slow_unique_key tl)
+  end.
+
+Lemma has_remove_key_all : forall {T} (x y : string * T) (li : list (string * T)),
+  fst_cmp x y = false ->
+  has_with fst_cmp x (remove_key_all (fst y) li) = has_with fst_cmp x li.
+Proof.
+  intros. generalize dependent y. generalize dependent x. induction li; intros; simpl in *. { reflexivity. }
+  destruct a. destruct x. destruct y. unfold fst_cmp in *. simpl in *.
+  destruct (eqb s1 s) eqn:E1. { apply eqb_eq in E1. subst. rewrite H. apply (IHli (s0, t0) (s, t)). assumption. }
+  destruct (eqb s0 s) eqn:E0; simpl in *. { rewrite E0. reflexivity. } rewrite E0. apply (IHli (s0, t0) (s1, t1)). assumption.
+Qed.
+
+Lemma has_slow_unique : forall {T} x li,
+  has_with (@fst_cmp T T) x (slow_unique_key li) = has_with fst_cmp x li.
+Proof.
+  intros T [s t] li. generalize dependent t. generalize dependent s.
+  induction li; intros; simpl in *. { reflexivity. }
+  destruct a. destruct (eqb_spec s s0). { subst. unfold fst_cmp. simpl. rewrite eqb_refl. reflexivity. }
+  simpl. rewrite (has_remove_key_all (s, t) (s0, t0)). 2: { unfold fst_cmp. simpl. apply eqb_neq. assumption. }
+  unfold fst_cmp. simpl. apply eqb_neq in n. rewrite n. apply IHli.
+Qed.
+
+Lemma dup_from_src_fst_nil : forall {T} (a : list (string * T)),
+  dup_from_src_with fst_cmp a [] = slow_unique_key a.
+Proof.
+  induction a; intros; simpl in *. { reflexivity. }
+  destruct a. rewrite IHa. destruct (has_with fst_cmp (s, t) (slow_unique_key a0)) eqn:Eh. Abort.
+
+Lemma dup_with_src_fst_app_exists : forall {T} a b, exists pre,
+  @dup_from_src_with (string * T) fst_cmp a b = pre ++ b.
+Proof.
+  induction a; intros; simpl in *. { exists []. reflexivity. }
+  destruct (IHa b) as [x H]. rewrite H. destruct (has_with fst_cmp a (x ++ b));
+  [exists x | exists (a :: x); simpl; f_equal]; reflexivity.
+Qed.
+
+Lemma has_fst_or : forall {T} x a b,
+  @has_with (string * T) (string * T) fst_cmp x (dup_from_src_with fst_cmp a b) =
+  orb (has_with fst_cmp x a) (has_with fst_cmp x b).
+Proof.
+  intros T x a. generalize dependent x. induction a; intros; simpl in *. { reflexivity. }
+  destruct (has_with fst_cmp a (dup_from_src_with fst_cmp a0 b)) eqn:Eh; simpl in *;
+  (destruct (fst_cmp x a) eqn:Ef; simpl in *; [| apply IHa]). 2: reflexivity.
+  destruct a. destruct x. rewrite has_cmp_fst in *.
+  unfold fst_cmp in Ef. simpl in *. apply eqb_eq in Ef. subst. assumption.
+Qed.
+
+Lemma dup_with_src_fst_app : forall {T} a b,
+  @dup_from_src_with (string * T) fst_cmp a b =
+  fold_left (fun acc x => remove_key_all (fst x) acc) b (slow_unique_key a) ++ b.
+Proof.
+  induction a; intros; simpl in *. {
+    rewrite <- (app_nil_l b). f_equal. simpl. induction b; simpl. { reflexivity. } apply IHb. }
+  destruct a. destruct (has_with fst_cmp (s, t) (dup_from_src_with fst_cmp a0 b)) eqn:Eh;
+  rewrite IHa; [| rewrite app_comm_cons]; f_equal.
+  - remember (dup_from_src_with fst_cmp a0 b) as d eqn:Ed. generalize dependent s. generalize dependent t.
+    generalize dependent a0. generalize dependent b. induction d; intros; simpl in *. { discriminate Eh. }
+    rewrite has_cmp_fst in Eh. apply has_in_iff in Eh; [| apply eqb_eq]. destruct Eh.
+    2: { apply IHl. rewrite has_cmp_fst. apply has_in_iff. { apply eqb_eq. } assumption. }
+    apply IHl.
+
+  - rewrite has_fst_or in Eh. apply Bool.orb_false_iff in Eh as [H1 H2]. rewrite has_cmp_fst in *.
+    induction b; simpl in *. f_equal. rewrite remove_key_all_eq.
+    + reflexivity.
+    + intro C. eapply has_in_iff in C; [| apply eqb_eq]. erewrite <- has_cmp_fst in C. Search (has_with eqb). { rewrite H1 in C. } Search remove_key_all.
+
+    + rewrite has_fst_or. rewrite Eh. simpl in *. rewrite IHa. f_equal. 
+    specialize (IHa b).
+    apply IHa.
+  destruct (IHa b) as [x H]. rewrite H. destruct (has_with fst_cmp a (x ++ b));
+  [exists x | exists (a :: x); simpl; f_equal]; reflexivity.
+Qed.
+
+Theorem grand_unified_subst_structural_id : forall t,
+  let P := fun p : _ * _ => let (x, f) := p in f (TmVarS x) = t in
+  Forall P (grand_unified_subst_with remove_key_all t).
+Proof.
+  induction t as [| | | | id arg a IHa b IHb | arg a IHa b IHb | a IHa b IHb];
+  subst; simpl in *; try solve [repeat constructor]; [| |
+    apply Forall_app; split; apply Forall_smap; (eapply Forall_impl; [| try apply IHa; apply IHb]);
+    intros; destruct a0; rewrite H; reflexivity];
+  simpl. Search dup_from_src_with.
+  remember (grand_unified_subst_with remove_key_all a) as g eqn:Eg; [generalize dependent id |];
+  generalize dependent arg; generalize dependent a; generalize dependent b; (
+    induction g; intros; simpl in *; [
+      apply Forall_smap; destruct arg; [eapply incl_Forall; [apply remove_key_all_incl |] |];
+      (eapply Forall_impl; [| apply IHb]); intros; destruct a0; rewrite H; reflexivity |]);
+  destruct a; simpl in *; rewrite has_cmp_fst; rewrite dup_from_src_fst; repeat rewrite map_fst_smap;
+  destruct arg.
+  - admit.
+  - specialize (IHg _ IHb). clear IHg IHb IHa Eg. simpl in *. Search (map fst). rewrite has_cmp_fst. Search (has_with fst_cmp).
+
 Theorem grand_unified_subst_id : forall t,
   let P := fun p : _ * _ => let (x, f) := p in f (TmVarS x) = t in
   Forall P (grand_unified_subst t).
 Proof.
+  induction t as [| | | | id arg a IHa b IHb | arg a IHa b IHb | a IHa b IHb];
+  subst; simpl in *; try solve [repeat constructor]; [| |
+    apply Forall_app; split; apply Forall_smap; (eapply Forall_impl; [| try apply IHa; apply IHb]);
+    intros; destruct a0; rewrite H; reflexivity];
+  repeat rewrite dup_from_src_fst. simpl in *.
+
   induction t as [| | | | id arg a IHa b IHb | arg a IHa b IHb | a IHa b IHb];
   subst; simpl in *; try solve [repeat constructor];
   apply Forall_app; split; apply Forall_smap; try destruct arg;
